---
title: "Week 14"
author: "Vivian Kong"
date: "5/1/2018"
output: html_document
---

Taylor series
I will find all of the Taylor series for the following practice around x=0  
1.$$ f(x)= \frac {1}{(1-x)} $$

$$  f(x)=\frac {1}{(1-x)}, f(0)=1$$
$$ f'(x)=(1-x)^{-2}, f(0)=1$$
$$ f''(x)=2(1-x)^{-3}, f(0)=2$$
$$ f'''(x)=6(1-x)^{-4}, f(0)=6$$
$$ f''''(x)=24(1-x)^{-5}, f(0)=24$$
Follow the patterns here, we find the Taylor Series for $$ f(x)=\frac {1}{1-x}= 1+x+ \frac{2x^2} {2!}+ \frac {6x^3} {3!}+ \frac{24x^4}{4!}+...$$

$$ f(x)= 1+x+x^2+x^3+x^4+...=\sum_{n=0}^{\infty} x^n $$

2. $$ f(x)= e^x $$

$$ f(x)=e^x, f(0)=1$$
$$ f'(x)=e^x, f'(0)=1$$
$$ f''(x)=e^x, f''(0)=1$$
$$ f'''(x)=e^x, f'''(0)=1$$
Follow the patterns, we find the Taylor series for $$ f(x)=e^x= 1+x+ \frac{x^2}{2!}+ \frac{x^3}{3!}+ \frac{x^4}{4!}+...= \sum_{n=0}^{\infty} \frac {x^n}{n!} $$

3. $$ f(x)=ln(1+x) $$
$$f(x)=ln(1+x), f(0)=0$$
$$ f'(x)=\frac {1}{1+x}, f'(0)=1$$
$$f''(x)=\frac {-1}{(1+x)^2}, f''(0)=-1$$
$$ f'''(x)=\frac {2}{(1+x)^3}, f'''(0)=2$$
$$ f''''(x)=\frac {-6}{(1+x)^4}, f''''(0)=-6$$

Follow the patterns, we find the Taylor series for $$f(x)= ln(1+x)= x- \frac {x^2} {2!}+ \frac {2x^3} {3!}- \frac {6x^4} {4!}=x- \frac{x^2}{2}+ \frac{x^3}{3}- \frac{x^4}{4}+...= \sum_{n=1}^{\infty} (-1)^{n+1}  \frac{x^n}{n}$$




